Foundation/Propositional/FMT/Hilbert/VF_Ser.lean
@@ -1,6 +1,6 @@
 module
 
-public import Foundation.Propositional.FMT.AxiomSer
+public import Foundation.Propositional.FMT.Axiom.Ser
 
 @[expose] public section
 
@@ -8,10 +8,7 @@ namespace LO.Propositional
 
 open FMT
 
-
 namespace FMT
-
-protected abbrev FrameClass.VF_Ser : FMT.FrameClass := { F | F.IsNTSerial }
 
 instance : trivialFrame.IsNTSerial where
   nt_serial := by tauto;
@@ -19,46 +16,43 @@ instance : trivialFrame.IsNTSerial where
 end FMT
 
 
-namespace VF_Ser
+namespace HilbertVF.VF_Ser
 
-open Hilbert.VF.FMT
+open HilbertVF.FMT
 open Formula.FMT
 
-
-instance FMT.sound : Sound Propositional.VF_Ser FrameClass.VF_Ser := by
+instance soundFMT : Sound HilbertVF.VF_Ser ({ F | F.IsNTSerial } : FMT.FrameClass) := by
   apply instFrameClassSound;
   constructor;
   rintro φ rfl F hF;
   replace hF := Set.mem_setOf_eq.mp hF;
   apply valid_axiomSer_of_isDNFSerial;
 
-instance : Entailment.Consistent Propositional.VF_Ser := consistent_of_sound_frameclass FrameClass.VF_Ser $ by
+instance : Entailment.Consistent (HilbertVF.VF_Ser : HilbertVF ℕ) := consistent_of_sound_frameclass ({ F | F.IsNTSerial } : FMT.FrameClass) $ by
   use FMT.trivialFrame;
   apply Set.mem_setOf_eq.mpr;
   infer_instance;
 
-instance FMT.complete : Complete Propositional.VF_Ser FrameClass.VF_Ser := by
+instance completeFMT : Complete HilbertVF.VF_Ser ({ F | F.IsNTSerial } : FMT.FrameClass) := by
   constructor;
   intro φ h;
   apply FMT.provable_of_validOnHintikkaModel;
   apply h;
   apply isDNFSerial_HintikkaModel;
 
-open Formula.FMT
-
-end VF_Ser
+end HilbertVF.VF_Ser
 
 open Formula.FMT in
 open Entailment.Corsi in
-instance : Propositional.VF ⪱ Propositional.VF_Ser := by
+instance : (HilbertVF.VF : HilbertVF ℕ) ⪱ HilbertVF.VF_Ser := by
   constructor;
-  . apply Hilbert.VF.weakerThan_of_subset_axioms;
+  . apply HilbertVF.weakerThan_of_le;
     tauto;
   . apply Entailment.not_weakerThan_iff.mpr;
     use Axioms.Ser;
     constructor;
     . simp;
-    . apply Sound.not_provable_of_countermodel (𝓜 := FMT.FrameClass.VF);
+    . apply HilbertVF.VF.soundFMT.not_provable_of_countermodel;
       apply FMT.not_validOnFrameClass_of_exists_model_world;
       use {
         World := Fin 2,
@@ -71,10 +65,8 @@ instance : Propositional.VF ⪱ Propositional.VF_Ser := by
       . tauto;
       . apply Formula.FMT.Forces.not_def_imp.mpr;
         use 1;
-        refine ⟨?_, ?_, ?_⟩;
-        . tauto;
-        . grind;
-        . tauto;
+        grind;
 
 end LO.Propositional
+
 end
